theories/CeresParserRoundtrip.v
@@ -85,6 +85,7 @@ Inductive list_tokens {A B} (tks : A -> list B -> Prop) : list A -> list B -> Pr
 | list_tokens_cons x xs y ys
   : tks x y -> list_tokens tks xs ys -> list_tokens tks (x :: xs) (y ++ ys)
 .
+Hint Constructors list_tokens : core.
 
 Inductive atom_token : atom -> Token.t -> Prop :=
 | atom_token_Raw s : atom_token (Raw s) (Token.Atom s)
@@ -98,7 +99,7 @@ Inductive sexp_tokens : sexp -> list Token.t -> Prop :=
   : list_tokens sexp_tokens es ts -> sexp_tokens (List es) (Token.Open :: ts ++ [Token.Close])
 .
 
-Definition list_sexp_tokens := list_tokens sexp_tokens.
+Notation list_sexp_tokens := (list_tokens sexp_tokens).
 
 (* * Lemmas *)
 
@@ -145,29 +146,60 @@ Definition escape_to_string (e : escape) : string :=
 Definition nonewline (s : string) : Prop.
 Admitted.
 
+Definition is_atom_string (s : string) : Prop.
+Admitted.
+
+Lemma is_atom_singleton (c : ascii)
+  : is_atom_char c = true -> is_atom_string (c :: "").
+Proof.
+Admitted.
+Hint Resolve is_atom_singleton : ceres.
+
+Lemma is_atom_app (s : string) (c : ascii)
+  : is_atom_string s -> is_atom_char c = true -> is_atom_string (s ++ c :: "").
+Proof.
+Admitted.
+Hint Resolve is_atom_app : ceres.
+
+Inductive str_token_string (tok : string) (e : escape) : string -> Prop :=
+| str_token_string_mk : str_token_string tok e ("""" :: string_reverse tok ++ escape_to_string e)
+.
+
 Inductive partial_token_string : partial_token -> string -> Prop :=
 | partial_token_string_NoToken
   : partial_token_string NoToken ""
-| partial_token_string_SimpleToken p s
-  : partial_token_string (SimpleToken p s) s
-| partial_token_string_StrToken p tok e
-  : partial_token_string (StrToken p tok e) ("""" :: string_reverse tok ++ escape_to_string e)
+| partial_token_string_SimpleToken p s s'
+  : is_atom_string s' ->
+    s' = string_reverse s ->
+    partial_token_string (SimpleToken p s) s'
+| partial_token_string_StrToken p tok e s'
+  : str_token_string tok e s' ->
+    partial_token_string (StrToken p tok e) s'
 | partial_token_string_Comment s
   : nonewline s ->
     partial_token_string Comment (";" :: s)
 .
 Hint Constructors partial_token_string : core.
 
+Inductive parser_state_string_
+    (more : bool) (d : list sexp) (u : list symbol) (s0 : string) : Prop :=
+| parser_state_string_mk_ ts00 ts01
+  : token_string more (ts00 ++ ts01) s0 ->
+    list_sexp_tokens d ts00 ->
+    stack_tokens u ts01 ->
+    parser_state_string_ more d u s0
+.
+Hint Constructors parser_state_string_.
+
 (* Invariant on the parsed prefix *)
 Inductive parser_state_string (i : parser_state) : string -> Prop :=
-| parser_state_string_mk more ts00 ts01 s0 s1
-  : token_string more (ts00 ++ ts01) s0 ->
+| parser_state_string_mk more s0 s1
+  : parser_state_string_ more (parser_done i) (parser_stack i) s0 ->
     more_ok more s1 ->
-    list_sexp_tokens (parser_done i) ts00 ->
-    stack_tokens (parser_stack i) ts01 ->
     partial_token_string (parser_cur_token i) s1 ->
     parser_state_string i (s0 ++ s1)
 .
+Hint Constructors parser_state_string.
 
 Definition on_right {A B} (x : A + B) (P : B -> Prop) : Prop :=
   match x with
@@ -187,66 +219,137 @@ Proof.
   induction s; [ auto | cbn; rewrite IHs; auto ].
 Qed.
 
+Lemma _fold_stack_sound_
+    d
+    (p : loc)
+    (s0 : string)
+    (more : bool)
+    u
+  : forall
+    (es : list sexp)
+    (ts00 ts01 ts02 : list Token.t)
+    (Hs0 : token_string more (ts00 ++ ts01 ++ ts02) s0)
+    (Hdone : list_sexp_tokens d ts00)
+    (Hstack : stack_tokens u ts01)
+    (Hes : list_sexp_tokens es ts02)
+  , on_right (_fold_stack d p es u)
+      (fun i' : parser_state => parser_state_string i' (s0 ++ ")")).
+Proof.
+  induction u; cbn; auto; intros.
+  destruct a; cbn.
+  - admit.
+  - inversion Hstack; subst; clear Hstack.
+    rewrite <- app_assoc in Hs0.
+    specialize IHu with (1 := Hs0).
+    apply IHu; auto.
+Admitted.
+
+Lemma _fold_stack_sound
+    d
+    (p : loc)
+    (s0 : string)
+    (more : bool)
+    u
+  : parser_state_string_ more d u s0 ->
+    on_right (_fold_stack d p [] u)
+      (fun i' : parser_state => parser_state_string i' (s0 ++ ")")).
+Proof.
+  intros [ts00 ts01 ? ?]; apply _fold_stack_sound_
+    with (more := more) (ts00 := ts00) (ts01 := ts01) (ts02 := []); auto.
+  rewrite app_nil_r; auto.
+Qed.
+
+Lemma next_sound' {T} (i : parser_state_ T) (more : bool) s0 p c
+  : parser_state_string_ more (parser_done i) (parser_stack i) s0 ->
+    on_right (next' i p c) (fun i' =>
+      parser_state_string i' (s0 ++ c :: "")).
+Proof.
+  intros [ts00 ts01 Hs0 Hdone Hstack].
+  unfold next'; match_ascii; cbn.
+  + (* "(" *)
+    rewrite <- (string_app_nil_r (_ ++ "(")).
+    apply parser_state_string_mk with (more := false); auto.
+    apply parser_state_string_mk_
+      with (ts00 := ts00) (ts01 := ts01 ++ [Token.Open]);
+      cbn; auto.
+    rewrite app_assoc; apply token_string_open_app with (more := more); eauto.
+  + (* ")" *)
+    eauto using _fold_stack_sound.
+  + (* """" *)
+    eapply parser_state_string_mk; cbn; eauto.
+    1,2: admit.
+  + (* ";" *)
+    eapply parser_state_string_mk; cbn; eauto.
+    1,2: admit.
+  + (* else *)
+    destruct (is_whitespace y) eqn:Ews; cbn.
+    * rewrite <- (string_app_nil_r (_ ++ y :: "")).
+      eapply parser_state_string_mk; cbn; eauto.
+      eapply parser_state_string_mk_; cbn; eauto.
+      admit.
+    * auto.
+Admitted.
+
+Lemma more_ok_atom more s c
+  : more_ok more s ->
+    is_atom_string s ->
+    is_atom_char c = true ->
+    more_ok more (s ++ c :: "").
+Proof.
+Admitted.
+Hint Resolve more_ok_atom : ceres.
+
+Lemma string_reverse_cons_ c s1 s'
+  : forall s0,
+    s' = _string_reverse s0 s1 ->
+    (s' ++ c :: "")%string = _string_reverse (s0 ++ c :: "") s1.
+Proof.
+  induction s1; cbn; intros s0 Hs0.
+  - f_equal; auto.
+  - apply IHs1 in Hs0; auto.
+Qed.
+
+Lemma string_reverse_cons c s s'
+  : s' = string_reverse s ->
+    (s' ++ c :: "")%string = string_reverse (c :: s)%string.
+Proof.
+  apply string_reverse_cons_.
+Qed.
+
+Lemma new_sexp_Atom_sound d u s0 ts00 ts01 more
+    (Hs0 : token_string more (ts00 ++ ts01) s0)
+    (Hdone : list_sexp_tokens d ts00)
+    (Hstack : stack_tokens u ts01)
+    (s' : string)
+    (Hmore : more_ok more s')
+    (s1' : string)
+    (H : is_atom_string s')
+    (H0 : s' = string_reverse s1')
+    (i' := new_sexp d u (Atom (raw_or_num s1')) tt)
+  : parser_state_string_ true (parser_done i') (parser_stack i') (s0 ++ s').
+Proof.
+Admitted.
+
 Lemma next_sound i s p c
   : parser_state_string i s ->
     on_right (next i p c) (fun i' =>
       parser_state_string i' (s ++ c :: "")).
 Proof.
-  intros [more ts00 ts01 s0 s1 Hs0 Hmore Hdone Hstack Hcur].
+  intros [more s0 s1 Hi Hmore Hcur].
   unfold next.
   destruct Hcur as [ | p1' s1' | p1 tok e | s1' Hs ].
   - (* NoToken *)
-    unfold next'.
     apply more_ok_nil_inv in Hmore; subst more.
     rewrite string_app_nil_r.
-    match_ascii; cbn.
-    + (* "(" *)
-      rewrite <- (string_app_nil_r (s0 ++ "(")).
-      apply parser_state_string_mk
-        with (more := false) (ts00 := ts00) (ts01 := ts01 ++ [Token.Open]);
-        cbn; auto.
-      rewrite app_assoc; eapply token_string_open_app; eauto.
-    + (* ")" *)
-      admit.
-    + (* """" (double quote char) *)
-      apply parser_state_string_mk
-        with (more := false) (ts00 := ts00) (ts01 := ts01);
-        cbn; auto.
-      constructor.
-    + (* ";" *)
-      apply parser_state_string_mk
-        with (more := false) (ts00 := ts00) (ts01 := ts01);
-        cbn; auto.
-      constructor.
-      admit.
-    + (* else *)
-      destruct (is_whitespace _) eqn:Hws; cbn.
-      * rewrite <- (string_app_nil_r (s0 ++ y :: "")).
-        apply parser_state_string_mk
-          with (more := false) (ts00 := ts00) (ts01 := ts01);
-          cbn; auto.
-        admit.
-      * admit.
+    destruct (is_atom_char c) eqn:IAC_c; cbn.
+    + econstructor; cbn; eauto with ceres.
+    + eauto using next_sound'.
   - (* SimpleToken *)
-    unfold next'.
-    match_ascii; cbn.
-    + (* "(" *)
-      rewrite <- (string_app_nil_r (_ ++ "(")).
-      apply parser_state_string_mk
-        with (more := false) (ts00 := ts00) (ts01 := ts01 ++ [Token.Open]);
-        cbn; auto.
-      * rewrite app_assoc; apply token_string_open_app with (more := true); eauto.
-        admit.
-      * admit.
-      * admit.
-    + (* ")" *)
-      admit.
-    + (* """" *)
-      admit.
-    + (* ";" *)
-      admit.
-    + (* else *)
-      admit.
+    destruct (is_atom_char c) eqn:IAC_c; cbn.
+    + rewrite string_app_assoc.
+      econstructor; cbn; eauto using string_reverse_cons with ceres.
+    + destruct Hi as [ts00 ts01 Hs0 Hdone Hstack].
+      eauto using next_sound', new_sexp_Atom_sound.
   - (* StrToken *)
     admit.
   - (* Comment *)
